Matrix Example uses machine integers now

Phi_Examples/PhiEx_Rational.C
@@ -1,0 +1,25 @@
+
+struct Rational {
+  int num, den;
+} ;
+
+struct Rational rat_add (struct Rational q1, struct Rational q2) {
+  return { num: q1.num * q2.den + q2.num * q1.den,
+           den: q1.den * q2.den };
+}
+
+struct Rational rat_sub (struct Rational q1, struct Rational q2) {
+  return { num: q1.num * q2.den - q2.num * q1.den,
+           den: q1.den * q2.den };
+}
+
+struct Rational rat_mul (struct Rational q1, struct Rational q2) {
+  return { num: q1.num * q2.num,
+           den: q1.den * q2.den };
+}
+
+struct Rational rat_div (struct Rational q1, struct Rational q2) {
+  return { num: q1.num * q2.den,
+           den: q1.den * q2.num };
+}
+
