Phi_Examples/time_distribution.py
@@ -10,7 +10,9 @@ pseudocount = 1
 reasoning = origin[:,0] / 1000.0
 proof_eval = origin[:,1] / 1000.0
 proof_search = origin[:,2]
-total = reasoning + proof_eval + proof_search
+total = origin[:,3]
+#total = 
+print (total - (reasoning + proof_eval + proof_search))
 
 proof_eval = proof_eval[proof_eval > 0.01]
 proof_search = proof_search[proof_search > 0]
@@ -20,26 +22,19 @@ log_proof_eval = np.log10(np.maximum(proof_eval, 10.0) + pseudocount)
 log_proof_search = np.log10(np.minimum(np.maximum(proof_search, 10.0), 3000000.0) + pseudocount)
 log_total = np.log10(total + pseudocount)
 
-tick_values = [10.0, 30.0, 100.0, 300.0, 500.0, 1000.0, 3000.0, 5000.0, 10000.0, 30000.0, 50000.0, 100000.0, 300000.0, 1000000]
-tick_names  = ['<0.01', '0.03', '0.1', '0.3  ', '  0.5', '1', '3', '5', '10', '30 ', ' 50', '100', '300', '1000']
+tick_values = [10.0, 30.0, 100.0, 300.0, 500.0, 1000.0, 3000.0, 5000.0, 10000.0, 30000.0, 100000.0, 300000.0, 1000000]
+tick_names  = ['<0.01    ', '0.03', '0.1', '0.3  ', '  0.5', '1', '3', '5', '10', '30 ', '100', '300', '1000']
 log_lower = np.log10(pseudocount + 10.0)
 log_upper = np.log10(pseudocount + 1000000.0)
 
 
-#def kde_boundary_corrected(data, label, linestyle, lower_bound, upper_bound):
-#    kde = sm.nonparametric.KDEUnivariate(data)
-#    kde.fit(bw='scott', fft=True, cut=0, gridsize=1000, clip=(lower_bound, upper_bound))
-#    plt.plot(kde.support, kde.density, label=label, color='black', linestyle=linestyle)
-
 def normalize_histogram(hist, bin_edges):
-    print (10 ** bin_edges - pseudocount)
-    print (hist)
-    return hist / sum(hist)
+    return hist / sum(hist) * 100.0
 
-log_hist1, log_bin_edges1 = np.histogram(log_reasoning, bins=50, range=(log_lower, log_upper))
-log_hist2, log_bin_edges2 = np.histogram(log_proof_eval, bins=50, range=(log_lower, log_upper))
-log_hist3, log_bin_edges3 = np.histogram(log_proof_search, bins=50, range=(log_lower, log_upper))
-log_hist4, log_bin_edges4 = np.histogram(log_total, bins=50, range=(log_lower, log_upper))
+log_hist1, log_bin_edges1 = np.histogram(log_reasoning, bins=30, range=(log_lower, log_upper))
+log_hist2, log_bin_edges2 = np.histogram(log_proof_eval, bins=30, range=(log_lower, log_upper))
+log_hist3, log_bin_edges3 = np.histogram(log_proof_search, bins=30, range=(log_lower, log_upper))
+log_hist4, log_bin_edges4 = np.histogram(log_total, bins=30, range=(log_lower, log_upper))
 
 log_hist1 = normalize_histogram (log_hist1, log_bin_edges1)
 log_hist2 = normalize_histogram (log_hist2, log_bin_edges2)
@@ -56,24 +51,16 @@ plot_hist_as_line(log_hist3, log_bin_edges3, 'proof search', '-.', '#610807')
 plot_hist_as_line(log_hist4, log_bin_edges4, 'total', '-', 'black')
 
 
-
-#def original_scale_log_formatter(val, pos):
-#    original_val = np.exp(val) - pseudocount
-#    return f'{original_val:.2f}'
-
-# KDE plots for the log10-transformed data
-#kde_boundary_corrected(log_reasoning, 'reasoning', '-', 0, 10000)
-#kde_boundary_corrected(log_proof_eval, 'proof eval', '--', 0, 10000)
-#sns.kdeplot(log_proof_search, label='proof search', color='black', linestyle='-.', shade=True)
-
 log_tick_positions = [np.log10(tick + pseudocount) for tick in tick_values]
 plt.xticks(log_tick_positions, tick_names)
 
-#XX = plt.gca().get_xaxis()
-#XX.set_major_formatter(tk.FuncFormatter(lambda x, p: format(int(x))))
+plt.xlabel('seconds')
+#plt.ylabel('Portion')
+ax = plt.gca()  # Get the current axis
+ax.yaxis.set_major_formatter(tk.PercentFormatter(decimals=0))
+ax.xaxis.set_label_coords(0.955, -0.025)
+ax.xaxis.label.set_bbox(dict(facecolor='white', edgecolor='none', pad=3))
 
-plt.xlabel('Time')
-plt.ylabel('Density')
 plt.legend()
 
 plt.grid(linestyle=':')
