Phi_Examples/transformation-opr-step.py
@@ -5,6 +5,15 @@ import pandas as pd
 import statsmodels.formula.api as smf
 from matplotlib.ticker import MaxNLocator
 
+
+from matplotlib import rc
+
+# Set up for using the desired fonts
+rc('font', family='Libertine', size=15)
+rc('text', usetex=True)
+rc('text.latex', preamble=r'\usepackage{libertine}\usepackage{newtxmath}')
+
+
 origin = np.genfromtxt("transformation-opr-step.csv", delimiter=",")
 X = origin[:,0]
 Y = origin[:,1]
@@ -20,18 +29,22 @@ x_range = np.linspace(X.min(), X.max(), 100)
 #y_fit = quantile_model_quad.params['Intercept'] + quantile_model_quad.params['X'] * x_range + quantile_model_quad.params['X2'] * x_range**2
 y_fit = quantile_model_quad.params['Intercept'] + quantile_model_quad.params['X'] * x_range #+ quantile_model_quad.params['X2'] * x_range**2
 
-plt.plot(x_range, y_fit, color='black', label='95th percentile regression line')
+plt.figure(figsize=(4.3, 2.9))
+plt.plot(x_range, y_fit, linestyle='--', linewidth=0.6, color='black', label=r'\parbox{7em}{95th percentile\\regression}')
 
 #plt.title('Scatter plot with high transparency')
 plt.scatter(X, Y, color='grey', alpha=0.2, edgecolors='none')
-plt.xlabel("# of type operators")
-plt.ylabel("LP steps")
+plt.xlabel("100 typ oprs")
+#plt.ylabel("LP steps")
+#ax.xaxis.set_label_coords(0.85, -0.045)
+#ax.xaxis.label.set_bbox(dict(facecolor='white', edgecolor='none', pad=3))
+#ax.xaxis.set_major_locator(MaxNLocator(nbins='auto'))
+plt.xticks([0,25,50,75,100], ['0','25','50','75', '100 typ oprs'])
 ax = plt.gca()  # Get the current axis
-ax.xaxis.set_label_coords(0.86, -0.025)
-ax.xaxis.label.set_bbox(dict(facecolor='white', edgecolor='none', pad=3))
-ax.xaxis.set_major_locator(MaxNLocator(nbins='auto'))
-plt.legend()
+ax.xaxis.get_majorticklabels()[3].set_horizontalalignment("right")
+plt.yticks([50,100,150,200,250])
 
+plt.legend(framealpha=0.1)
 #plt.tight_layout()
 plt.show()
 
